\documentclass[12pt]{article}
\linespread{1.2}
\usepackage[margin=2cm]{geometry}
\usepackage[utf8]{inputenc}
\usepackage{amsfonts}
\usepackage{amsmath}
\usepackage{multicol}
\usepackage{amsthm}
\usepackage{amssymb,scrextend}
\usepackage{graphicx,tikz,pgfplots}
\pgfplotsset{compat=1.18}
\newtheorem{dfn}{Definition}
\renewcommand{\qed}{\hfill$\blacksquare$}
\let\newproof\proof
\renewenvironment{proof}{\vspace{1em}\begin{addmargin}[2em]{0em}\begin{newproof}}{\end{newproof}\end{addmargin}\qed}
\newenvironment{theorem}[2][Theorem]{\begin{trivlist}
\item[\hskip \labelsep {\bfseries #1} \hskip \labelsep {\bfseries #2.}]}{\end{trivlist}}
\newenvironment{example}[2][Example]{\begin{trivlist}
\item[\hskip \labelsep {\bfseries #1} \hskip \labelsep {\bfseries #2.}]}{\end{trivlist}}
\newenvironment{lemma}[2][Lemma]{\begin{trivlist}
\item[\hskip \labelsep {\bfseries #1} \hskip \labelsep {\bfseries #2.}]}{\end{trivlist}}
\newenvironment{exercise}[2][Exercise]{\begin{trivlist}
\item[\hskip \labelsep {\bfseries #1} \hskip \labelsep {\bfseries #2.}]}{\end{trivlist}}
\newenvironment{problem}[2][Problem]{\begin{trivlist}
\item[\hskip \labelsep {\bfseries #1} \hskip \labelsep {\bfseries #2.}]}{\end{trivlist}}
\newenvironment{corollary}[2][Corollary]{\begin{trivlist}
\item[\hskip \labelsep {\bfseries #1} \hskip \labelsep {\bfseries #2.}]}{\end{trivlist}}
\usepackage{fancyhdr,enumitem,changepage,url}
\pagestyle{fancy}
\author{Warren Atkison}
\date{\today}
\setlength{\headheight}{15pt}
\begin{document}
\fancyhf{}
\fancyhead[L]{Warren Atkison}
\fancyhead[C]{Homework Set 2.1}
\fancyhead[R]{\today}
\fancyfoot[R]{\thepage}

\begin{exercise}{4c} 
	Show that the inversion mapping $w = f(z) = 1/z$ maps the circle $|z - 1| = 1$ onto the verticle line $x = 1/2$
\begin{proof} Let $z = x + iy$
	\begin{multicols}{2}	
	\begin{align*}
		1 = |z - 1|^2 &= (z - 1)\overline{(z - 1)} \\
			      &= (z - 1)(\overline{z} - 1) \\
			      &= z\overline{z} -z -\overline{z} + 1 \\
			      &= |z|^2 - 2x + 1 \\
		\implies |z|^2 &= 2x \\
	\end{align*}
	\begin{align*}
		\\
		w = \frac{1}{x + iy}&= \frac{x - iy}{x^2 + y^2} \\
				     &= \frac{x}{|z|^2} - \frac{iy}{|z|^2} \\
								&= \frac{x}{2x} - \frac{iy}{|z|^2} \\
								&= \frac{1}{2} - \frac{iy}{|z|^2}
	\end{align*}
	\end{multicols}
\end{proof}	
\end{exercise}
\begin{exercise}{6c}
	The \textit{Joukowski mapping} is defined by
	\[
		w = J(z) = \frac{1}{2}\left(z + \frac{1}{z}\right).
	\]
	Show that $J$ maps the circle $|z| = r$ $(r > 0,~r \neq 1)$ onto the ecliplse
	\[
		\dfrac{u^2}{\left[\dfrac{1}{2}\left(r + \dfrac{1}{r}\right)\right]^2} + \dfrac{v^2}{\left[\dfrac{1}{2}\left(r - \dfrac{1}{r}\right)\right]^2} = 1,
	\]
	where $J(z) = u + iv$.
	\begin{proof} Let $z = x + iy$
		\begin{align*}
			J(z) &= \frac{1}{2}\left(x + iy + \frac{1}{x + iy}\right) \\
			     &= \frac{1}{2}\left(x + iy + \frac{x}{r^2} - \frac{iy}{r^2}\right) \\
			     &= \frac{x}{2}\left(1 + \frac{1}{r^2}\right) + \frac{iy}{2}\left(1 - \frac{1}{r^2}\right) = u + iv
		\end{align*}
		\begin{align*}
			u &= \frac{x}{2}\left(1 + \frac{1}{r^2}\right) & v &= \frac{y}{2}\left(1 - \frac{1}{r^2}\right) \\
			x &= \dfrac{u}{\dfrac{1}{2}\left(1 + \dfrac{1}{r^2}\right)} & y &= \dfrac{v}{\dfrac{1}{2}\left(1 - \dfrac{1}{r^2}\right)}
		\end{align*}
		\begin{align*}
			|z|^2 = x^2 + y^2 = \dfrac{u^2}{\left[\dfrac{1}{2}\left(1 + \dfrac{1}{r^2}\right)\right]^2} + \dfrac{v^2}{\left[\dfrac{1}{2}\left(1 - \dfrac{1}{r^2}\right)\right]^2} &= r^2 \\		
			\dfrac{u^2}{r^2\left[\dfrac{1}{2}\left(1 + \dfrac{1}{r^2}\right)\right]^2} + \dfrac{v^2}{r^2\left[\dfrac{1}{2}\left(1 - \dfrac{1}{r^2}\right)\right]^2} &= 1 \\
			\dfrac{u^2}{\left[\dfrac{1}{2}\left(r + \dfrac{1}{r}\right)\right]^2} + \dfrac{v^2}{\left[\dfrac{1}{2}\left(r - \dfrac{1}{r}\right)\right]^2} &= 1
		\end{align*}
	\end{proof}
\end{exercise}
\begin{exercise}{8}
	A function of the form $G(z) = e^{i\phi}z$, where $\phi$ is a real constant, generates a \textit{rotation mapping}. Sketch the image of the semidisk $|z| \le 2$, $\Im z \ge 0$, under $G$ when \textbf{(a)} $\phi= \pi/4$; \textbf{(b)} $\phi = -\pi/4$; \textbf{(c)} $\pi = 3\pi/4$.
\end{exercise}	
\begin{center}
	\begin{tikzpicture}[scale = 0.8]
		\begin{axis}[xmin = -3, xmax = 3, ymin = -3, ymax = 3, axis x line = middle, axis y line = middle]
			\addplot[domain=0:2] {(4 - x^2)^(1/2)};		
			\addplot[domain=-2:0] {(4 - x^2)^(1/2)};
		\end{axis}
	\end{tikzpicture}
\end{center}
Let $z = re^{i\theta}$, then
\[
	G(z) = re^{i(\phi + \theta)}
\]

\begin{itemize}
	\begin{multicols}{3}
	\item[(a)] $G(z) = re^{i(\theta + \pi/4)}$ \\
		\begin{tikzpicture}[scale = 0.7]
			\begin{axis}[xmin = -3, xmax = 3, ymin = -3, ymax = 3, axis x line = middle, axis y line = middle]
				\addplot[domain=0:1.414214] {(4 - x^2)^(1/2)};		
				\addplot[domain=-2:0] {(4 - x^2)^(1/2)};
				\addplot[domain=-2:-1.414214] {-(4 - x^2)^(1/2)};
				\addplot[domain=-1.414214:1.414214] {x};
			\end{axis}
		\end{tikzpicture}
	\item[(b)] $G(z) = re^{i(\theta - \pi/4)}$ \\
		\begin{tikzpicture}[scale = 0.7]
			\begin{axis}[xmin = -3, xmax = 3, ymin = -3, ymax = 3, axis x line = middle, axis y line = middle]
				\addplot[domain=0:2] {(4 - x^2)^(1/2)};		
				\addplot[domain=-1.414124:0] {(4 - x^2)^(1/2)};
				\addplot[domain=1.414124:2] {-(4 - x^2)^(1/2)};
				\addplot[domain=-1.414214:1.414214] {-x};
			\end{axis}
		\end{tikzpicture}
	\item[(c)] $G = re^{i(\theta + 3\pi/4)}$ \\
		\begin{tikzpicture}[scale = 0.7]
			\begin{axis}[xmin = -3, xmax = 3, ymin = -3, ymax = 3, axis x line = middle, axis y line = middle]
				\addplot[domain=0:1.414214] {-(4 - x^2)^(1/2)};		
				\addplot[domain=-2:0] {-(4 - x^2)^(1/2)};
				\addplot[domain=-2:-1.414214] {(4 - x^2)^(1/2)};
				\addplot[domain=-1.414214:1.414214] {-x};
			\end{axis}
		\end{tikzpicture}
	\end{multicols}
\end{itemize}
\end{document}
