\documentclass[12pt]{article}
\linespread{1.2}
\usepackage[margin=2cm]{geometry}
\usepackage[utf8]{inputenc}
\usepackage{amsfonts}
\usepackage{amsmath}
\usepackage{multicol}
\usepackage{amsthm}
\usepackage{amssymb,scrextend}
\usepackage{graphicx,tikz}
\newtheorem{dfn}{Definition}
\renewcommand{\qed}{\hfill$\blacksquare$}
\let\newproof\proof
\renewenvironment{proof}{\vspace{1em}\begin{addmargin}[2em]{0em}\begin{newproof}}{\end{newproof}\end{addmargin}\qed}
\newenvironment{theorem}[2][Theorem]{\begin{trivlist}
\item[\hskip \labelsep {\bfseries #1} \hskip \labelsep {\bfseries #2.}]}{\end{trivlist}}
\newenvironment{example}[2][Example]{\begin{trivlist}
\item[\hskip \labelsep {\bfseries #1} \hskip \labelsep {\bfseries #2.}]}{\end{trivlist}}
\newenvironment{lemma}[2][Lemma]{\begin{trivlist}
\item[\hskip \labelsep {\bfseries #1} \hskip \labelsep {\bfseries #2.}]}{\end{trivlist}}
\newenvironment{exercise}[2][Exercise]{\begin{trivlist}
\item[\hskip \labelsep {\bfseries #1} \hskip \labelsep {\bfseries #2.}]}{\end{trivlist}}
\newenvironment{problem}[2][Problem]{\begin{trivlist}
\item[\hskip \labelsep {\bfseries #1} \hskip \labelsep {\bfseries #2.}]}{\end{trivlist}}
\newenvironment{corollary}[2][Corollary]{\begin{trivlist}
\item[\hskip \labelsep {\bfseries #1} \hskip \labelsep {\bfseries #2.}]}{\end{trivlist}}
\usepackage{fancyhdr,enumitem,changepage,url}
\pagestyle{fancy}
\author{Warren Atkison}
\date{\today}
\setlength{\headheight}{15pt}
\begin{document}
\fancyhf{}
\fancyhead[L]{Warren Atkison}
\fancyhead[C]{Homework Set 3.5}
\fancyhead[R]{\today}
\fancyfoot[R]{\thepage}

\begin{exercise}{10}
	Show that all the solutions of the equation $\cos z = 2i$ are given by $\pi/2 + 2k\pi - i\text{Log}(\sqrt{5} + 2)$, $-\pi/2 + 2k\pi + i\text{Log}(\sqrt{5}+2)$, for $k = 0,\pm1,\pm2,\ldots$.	
\end{exercise}	
\begin{proof} We can use the definition of $\cos^{-1}$ to find $z$.
	\begin{align*}
		\cos z = 2i \implies z &= \cos^{-1}(2i) \\
				       &= -i\log[2i + ((2i)^2 - 1)^{1/2}] \\
				       &= -i\log[i(2 \pm \sqrt{5})] \\
				       &= -i(\log(i) +1\text{Log}(2 \pm \sqrt{5})) \\
				       &= \pi/2 + 2k\pi -i\text{Log}(2 \pm \sqrt{5}) \text{ for } k = 0,\pm1,\pm2,\ldots
	\end{align*}
	Then when we choose the positive square root,
	\[
		z = \pi/2 + 2k\pi -i\text{Log}(2 + \sqrt{5}) \text{ for } k = 0,\pm1,\pm2,\ldots
	\]
	When we choose the negative square root, consider the following identity
	\[
		\frac{-1}{2 + \sqrt{5}} = \frac{-1}{2 + \sqrt{5}}\cdot\frac{2 - \sqrt{5}}{2 - \sqrt{5}} = 2 - \sqrt{5}.
	\]
	Then,
	\begin{align*}
		z &= \pi/2 + 2k\pi -i\text{Log}[-(2 + \sqrt{5})^{-1}] \text{ for } k = 0,\pm1,\pm2,\ldots \\
		  &= \pi/2 + 2k\pi + i\text{Log}(2 + \sqrt{5}) - i\log(-1) \\
		  &= 3\pi/2 + 2k\pi + i\text{Log}(2 + \sqrt{5}) \\
		  &= -\pi/2 + 2k\pi + i\text{Log}(2 + \sqrt{5})
	\end{align*}
\end{proof}
\begin{exercise}{19}
	Determine the inverse of the function, $q(z) = 2e^z + e^{2z}$
	explicitly in terms of the complex logarithm. Find \textit{all} values of $z$ for which $q(z) = 3$.
\end{exercise}	
\begin{align*}
	2e^z + e^{2z} &= w \implies e^{2z} + 2e^{z} - w = 0 \\
	e^{z} &= \frac{-2 \pm\sqrt{4 + 4w}}{2} = -1 \pm \sqrt{1 + w} \\
	z &= \log\left(-1 \pm \sqrt{1 + w}\right)
\end{align*}
\[
	q^{-1}(z) = \log\left(-1 \pm \sqrt{1 + z}\right).
\]
When $q(z) = 3$,
\begin{align*}
	q^{-1}(3) = \log(-1 \pm \sqrt{4}) = \log(-1 \pm 2)
\end{align*}
When we take $+2$,
\[
	q^{-1}(3) = \text{Log}(1) = 0
\]
When we take $-2$,
\begin{align*}
	q^{-1}(3) = \log(-3) = \text{Log}(3) + i\pi + 2k\pi \text{ for } k = 0,\pm1,\pm2,\ldots
\end{align*}
\end{document}
