\documentclass[12pt]{article}
\linespread{1.2}
\usepackage[margin=2cm]{geometry}
\usepackage[utf8]{inputenc}
\usepackage{amsfonts}
\usepackage{amsmath}
\usepackage{multicol}
\usepackage{amsthm}
\usepackage{amssymb,scrextend}
\usepackage{graphicx,tikz}
\newtheorem{dfn}{Definition}
\renewcommand{\qed}{\hfill$\blacksquare$}
\let\newproof\proof
\renewenvironment{proof}{\vspace{1em}\begin{addmargin}[2em]{0em}\begin{newproof}}{\end{newproof}\end{addmargin}\qed}
\newenvironment{theorem}[2][Theorem]{\begin{trivlist}
\item[\hskip \labelsep {\bfseries #1} \hskip \labelsep {\bfseries #2.}]}{\end{trivlist}}
\newenvironment{example}[2][Example]{\begin{trivlist}
\item[\hskip \labelsep {\bfseries #1} \hskip \labelsep {\bfseries #2.}]}{\end{trivlist}}
\newenvironment{lemma}[2][Lemma]{\begin{trivlist}
\item[\hskip \labelsep {\bfseries #1} \hskip \labelsep {\bfseries #2.}]}{\end{trivlist}}
\newenvironment{exercise}[2][Exercise]{\begin{trivlist}
\item[\hskip \labelsep {\bfseries #1} \hskip \labelsep {\bfseries #2.}]}{\end{trivlist}}
\newenvironment{problem}[2][Problem]{\begin{trivlist}
\item[\hskip \labelsep {\bfseries #1} \hskip \labelsep {\bfseries #2.}]}{\end{trivlist}}
\newenvironment{corollary}[2][Corollary]{\begin{trivlist}
\item[\hskip \labelsep {\bfseries #1} \hskip \labelsep {\bfseries #2.}]}{\end{trivlist}}
\usepackage{fancyhdr,enumitem,changepage,url}
\pagestyle{fancy}
\author{Warren Atkison}
\date{\today}
\setlength{\headheight}{15pt}
\begin{document}
\fancyhf{}
\fancyhead[L]{Warren Atkison}
\fancyhead[C]{Homework Set 6.4}
\fancyhead[R]{\today}
\fancyfoot[R]{\thepage}

\begin{exercise}{6.3.2}
	Verify the following integral formula by comparing it to the improper integral in Example 2.
	\[
		\text{p.v.} \int_{-\infty}^{\infty} \frac{x^2}{(x^2 + 9)^2}dx = \frac{\pi}{6}
	\]
\end{exercise}

Consider the function
\[
	g(x) = \frac{x^2}{(x^2 + 1)^2}.
\]

From Example 2 we know p.v.$\int_{\infty}^{\infty} g(x)dx = \pi/2$. Let $x = 3u$, then
\begin{align*}
	\frac{x^2}{(x^2 + 9)^2} &= \frac{9u^2}{(9u^2 + 1)^2} \\
				&= \frac{9u^2}{9(3u^2 + 1/3)^2} \\
				&= \frac{u^2}{(3u^2 + 1/3)^2} \cdot \frac{(1/3)^2}{(1/3)^2} \\
				&= \frac{1}{9}\cdot \frac{u^2}{(u^2 + 1)} \\
				&= \frac{1}{9}g(u)
\end{align*}

and $dx = 3du$. Then we have
\begin{align*}
	\text{p.v.}\int_{-\infty}^{\infty} \frac{x^2}{(x^2 + 9)^2}dx &= \frac{1}{3}\text{p.v.} \int_{-\infty}^{\infty} g(u)du \\
								     &= \frac{1}{3}\cdot\frac{\pi}{2} \\
								     &= \frac{\pi}{6}
\end{align*}

\begin{exercise}{6.4.3}
	Using the method of residue, verify the integral formula.
	\[
		\text{p.v.}\int_{0}^{\infty} \frac{\cos(x)}{(x^2 + 1)^2}dx = \frac{\pi}{2e}
	\]
\end{exercise}

Since $\cos(x) = \cos(-x)$, we have
\[
	\text{p.v.}\int_{0}^{\infty} \frac{\cos(x)}{(x^2 + 1)^2}dx = \text{p.v.}\int_{-\infty}^{0} \frac{\cos(x)}{(x^2 + 1)^2}dx
\]

and
\[
	\text{p.v.}\int_{0}^{\infty} \frac{\cos(x)}{(x^2 + 1)^2}dx = \frac{1}{2}\left(\text{p.v.}\int_{-\infty}^{\infty} \frac{\cos(x)}{(x^2 + 1)^2}dx	\right)
\]

Now we can break up the integral as follows,
\[
	\text{p.v.}\int_{-\infty}^{\infty} \frac{\cos(x)}{(x^2 + 1)^2}dz = \text{p.v.}\int_{-\infty}^{\infty} \frac{e^{ix}}{2(x^2 + 1)^2}dx + \text{p.v.}\int_{-\infty}^{\infty} \frac{e^{-ix}}{2(x^2 + 1)^2}dx.
\]

Let $f_1(z) = \dfrac{e^{iz}}{2(z^2 + 1)^2}$. Then
\begin{align*}
	\int_{\Gamma_{\rho}} f_1(z)dz &= \int_{-\rho}^{\rho} f_1(x)dx + \int_{C_{\rho}^{+}}f_1(z)dz. 
\end{align*}

We encounter singularities at $z = \pm i$, and because
\[
	|f_1(z)| = |f_1(x + iy)| = \frac{\left|e^{ix}\cdot e^{-y}\right|}{2|z^2 + 1|^2} = \frac{e^{-y}}{2|z^2 + 1|^2}
\]

we have in the upper half plane $(y \ge 0)$
\[
	|f_1(z)| \le \frac{1}{2|z^2 + 1|^2}.
\]

Thus for any $\rho > 1$, the integral over $C_{\rho}^{+}$ is bounded by
\[
	\left|\int_{C_{\rho}^{+}} f_1(z)dz\right| \le  \frac{\pi \rho}{2(\rho^2 - 1)^2}
\]

which goes to zero as $\rho \to \infty$. Since $+i$ is the only singularity in the upper half plane, we have for $\rho > 1$

\[
	\int_{-\rho}^{\rho} f_1(x)dz + \int_{-\rho}^{\rho} f_1(z)dz = 2\pi i \text{Res}(f_1; i).
\]

Hence on taking the limit as $\rho \to \infty$ we get
\[
	\text{p.v.}\int_{\infty}^{\infty} \frac{e^{ix}}{2(x^2 + 1)^2}dx + 0 = 2\pi i\text{Res}(f_1; i).
\]

But
\begin{align*}
	\text{Res}(f_1; i) &= \lim_{z \to i} \frac{d}{dz} [(z - i)^2f_1(z)] \\
			   &= \lim_{z \to i} \frac{d}{dz} \frac{e^{iz}}{2(z + i)^2} \\
			   &= \frac{-8\cdot(i/e) - (1/e)\cdot8i}{64} \\
			   &= \frac{-i}{4e}
\end{align*}

so
\[
	\text{p.v.}\int_{\infty}^{\infty} \frac{e^{ix}}{2(x^2 + 1)^2}dx = \frac{\pi}{2e}
\]

Let $f_2(z) = \dfrac{e^{-iz}}{2(z^2 + 1)^2}$, whose singularities coincide with $f_1$. Then
\[
	\left|\int_{C_{\rho}^{-}} f_2(z)dz\right| \le  \frac{\pi \rho}{2(\rho^2 - 1)^2}
\]

is also satisfied by the same argument for $f_1$. However, since we are moving from $\rho \to -\rho$, we are going in the negative direction so

\[
	\int_{-\rho}^{\rho} f_2(x)dz + \int_{-\rho}^{\rho} f_2(z)dz = -2\pi i \text{Res}(f_2; -i).	
\]

and as $\rho \to \infty$ we get

\begin{align*}
	\text{p.v.}\int_{\infty}^{\infty} \frac{e^{-ix}}{2(x^2 + 1)^2}dx + 0 &= -2\pi i\text{Res}(f_2; -i). \\
									     &= -2\pi i \lim_{z \to -i} \frac{d}{dz}[(z + i)^2f_2(z)] \\
									     &= -2\pi i \left(\frac{-8\cdot(-i/e) - (1/e)\cdot(-8i)}{64}\right) \\
									     &= -2\pi i\left(\frac{i}{4e}\right) \\
									     &= \frac{\pi}{2e}
\end{align*}

Therefore
\[
	\text{p.v.}\int_{-\infty}^{\infty} \frac{\cos(x)}{(x^2 + 1)^2}dx = \frac{\pi}{2e} + \frac{\pi}{2e} = \frac{\pi}{e}
\]

and
\[
	\text{p.v.}\int_{0}^{\infty} \frac{\cos(x)}{(x^2 + 1)^2}dx = \frac{\pi}{2e}	
\]
\end{document}
