\documentclass[12pt]{article}
\linespread{1.2}
\usepackage[margin=2cm]{geometry}
\usepackage[utf8]{inputenc}
\usepackage{amsfonts}
\usepackage{amsmath}
\usepackage{multicol}
\usepackage{amsthm}
\usepackage{amssymb,scrextend}
\usepackage{graphicx,tikz,pgfplots}
\pgfplotsset{compat=1.18}
\newtheorem{dfn}{Definition}
\renewcommand{\qed}{\hfill$\blacksquare$}
\let\newproof\proof
\renewenvironment{proof}{\vspace{0em}\begin{addmargin}[2em]{0em}\begin{newproof}}{\end{newproof}\end{addmargin}\qed}
\newenvironment{theorem}[2][Theorem]{\begin{trivlist}
\item[\hskip \labelsep {\bfseries #1} \hskip \labelsep {\bfseries #2.}]}{\end{trivlist}}
\newenvironment{example}[2][Example]{\begin{trivlist}
\item[\hskip \labelsep {\bfseries #1} \hskip \labelsep {\bfseries #2.}]}{\end{trivlist}}
\newenvironment{lemma}[2][Lemma]{\begin{trivlist}
\item[\hskip \labelsep {\bfseries #1} \hskip \labelsep {\bfseries #2.}]}{\end{trivlist}}
\newenvironment{exercise}[2][Exercise]{\begin{trivlist}
\item[\hskip \labelsep {\bfseries #1} \hskip \labelsep {\bfseries #2.}]}{\end{trivlist}}
\newenvironment{problem}[2][Problem]{\begin{trivlist}
\item[\hskip \labelsep {\bfseries #1} \hskip \labelsep {\bfseries #2.}]}{\end{trivlist}}
\newenvironment{corollary}[2][Corollary]{\begin{trivlist}
\item[\hskip \labelsep {\bfseries #1} \hskip \labelsep {\bfseries #2.}]}{\end{trivlist}}
\usepackage{fancyhdr,enumitem,changepage,url}
\pagestyle{fancy}
\author{Warren Atkison}
\date{\today}
\setlength{\headheight}{15pt}
\begin{document}
\fancyhf{}
\fancyhead[L]{Warren Atkison}
\fancyhead[C]{Special Problem Set 1}
\fancyhead[R]{\today}
\fancyfoot[R]{\thepage}

\begin{problem}{1}
	Suppose that $|\alpha| < 1$ and $\left|\frac{z - \alpha}{1 - \overline{\alpha} z}\right| \le 1$ where $z,~\alpha \in \mathbb{C}$. Prove that $|z| \le 1$.
\end{problem}
\begin{proof}
	\begin{align*}
		\left|\frac{z - \alpha}{1 - \overline{\alpha} z}\right| \le 1 \implies |z - \alpha| \le |1 - \overline{\alpha} z|
	\end{align*}
 	Recall that $|z| - |w| \le |z - w|$ and $|z - w| \le |z| + |w|$ (1.3.15) by the triangle inequality.
	\begin{align*}
		|z| - |\alpha| &\le |z - \alpha| \\ 
			       &\le |1 - \overline{\alpha} z| \\ 
			       &\le 1 + |\overline{\alpha} z | \\  
			       &\le 1 + |\alpha| |z|\\ 
		|z| - |\alpha| |z| &\le 1 + |\alpha| \\
		|z|(1 - |\alpha|) &\le 1 + |\alpha| \\
		|z| |1 - \alpha| &\le 1 + |\alpha| \\
		|z|(1 + |\alpha|) &\le 1 + |\alpha| \\
		|z| &\le 1 
	\end{align*}
\end{proof}
\begin{problem}{2}
	Let $P$ be a polynomial defined by $P(x) = z^2 + iz + 3 - 2i$. Find $P(w)$, where $w = 10i/(2+i)$. Write the answer in $a + bi$ form and include intermediate steps.
\end{problem}	
\begin{align*}
	w = \frac{10i}{2 + i} = \frac{10i(2 - i)}{5} = 2i(2 - i) = 2 + 4i
\end{align*}
\begin{align*}
	P(w) &= (2 + 4i)^2 + i(2 + 4i) + 3 - 2i \\
	     &= (-12 + 16i) + (-4 + 2i) + 3 - 2i \\
	     &= -13 + 16i
\end{align*}
\begin{problem}{3}
	Describe carefully and fully the set of all complex numbers that satisfy the equation $|z - i| = 2|z - 1|$.
\end{problem}	
Let $z = x+iy$.
\begin{align*}
	|x + iy - i| &= 2|x + iy - 1| \\
	x^2 + (y - 1)^2 &= 2(x - 1)^2 + 2y^2 \\
	x^2 - (2x^2 - 4x + 2) &= 2y^2 - (y^2 - 2y + 1) \\
	-x^2 + 4x - 2 &= y^2 + 2y - 1 \\
	x(4-x) &= y^2 + 2y + 1 \\
	&= (y + 1)^2 \\
	y &= \pm\sqrt{x(4 - x)} - 1
\end{align*}
All complex numbers which lie on this parabola satisfy the equation $|z-i| = 2|z - 1|$.
\begin{center}
	\begin{tikzpicture}
		\begin{axis}[xmin = 0, xmax = 10, ymin = -5, ymax = 5, axis x line = middle, axis y line = middle]
			\addplot[domain=4:10] {(x*(x-4))^(1/2) - 1};
			\addplot[domain=4:10] {-(x*(x-4))^(1/2) - 1};
		\end{axis}
	\end{tikzpicture}
\end{center}
\begin{problem}{4}
	Prove the following identity.
	\[
		\sin \theta + \sin 2\theta + \ldots + \sin n\theta = \frac{\sin(n\theta/2)\sin((n+1)\theta/2)}{\sin(\theta/2)}\text{, where } 0 < \theta < 2\pi
	\]
\end{problem}
\begin{proof}
	Let $z = e^{i\theta}$.
\begin{align*}
	1 + z + z^2 + \ldots + z^n &= \frac{z^{n+1} - 1}{z - 1} \\
				   &= \frac{z^{(n+1)/2}(z^{(n+1)/2} - \overline{z}^{(n+1)/2})}{z^{1/2}(z^{1/2} - \overline{z}^{1/2})} \\
				  &= \frac{z^{(n+1)/2}}{z^{1/2}}\cdot \frac{\sin((n+1)\theta/2)}{\sin(\theta/2)}
\end{align*}
\begin{align*}
	\sin \theta + \sin 2\theta + \ldots + \sin n\theta &= \frac{z - \overline{z}}{2i} + \frac{z^2 - \overline{z}^2}{2i} + \ldots + \frac{z^n - \overline{z}^n}{2i} \\
							   &= \frac{z + z^2 + \ldots + z^n - (\overline{z} + \overline{z}^2 + \ldots + \overline{z}^n)}{2i} \\
							   &= \left(\frac{z^{n+1} - 1}{z - 1} - 1 - \frac{\overline{z}^{n+1} - 1}{\overline{z} - 1} + 1 \right)/2i \\
							   &= \left(\frac{z^{(n+1)/2}}{z^{1/2}}\cdot\frac{\sin((n+1)\theta/2)}{\sin(\theta/2)} - \frac{\overline{z}^{(n+1)/2}}{\overline{z}^{1/2}}\cdot\frac{\sin((n+1)\theta/2)}{\sin(\theta/2)}\right)/2i \\
							   &= \left(\frac{\sin((n+1)\theta/2)}{\sin(\theta/2)}\right)\left(\frac{z^{(n+1)/2}}{z^{1/2}} - \frac{\overline{z}^{(n+1)/2}}{\overline{z}^{1/2}}\right)/2i \\
							   &= \left(\frac{\sin((n+1)\theta/2)}{\sin(\theta/2)}\right)\left(\frac{z^{-1/2}z^{(n+1)/2} - z^{1/2}z^{-(n+1)/2}}{z^{1/2}z^{-1/2}}\right)/2i \\
							   &= \left(\frac{\sin((n+1)\theta/2)}{\sin(\theta/2)}\right)\left(\frac{z^{n/2} - z^{-n/2}}{2i}\right) \\
							   &= \frac{\sin(n\theta/2)\sin((n+1)\theta/2)}{\sin(\theta/2)}
\end{align*}
\end{proof}
\end{document}
