\documentclass[12pt]{article}
\linespread{1.2}
\usepackage[margin=2cm]{geometry}
\usepackage[utf8]{inputenc}
\usepackage{amsfonts}
\usepackage{amsmath}
\usepackage{multicol}
\usepackage{amsthm}
\usepackage{amssymb,scrextend}
\usepackage{graphicx,tikz}
\newtheorem{dfn}{Definition}
\renewcommand{\qed}{\hfill$\blacksquare$}
\let\newproof\proof
\renewenvironment{proof}{\vspace{1em}\begin{addmargin}[2em]{0em}\begin{newproof}}{\end{newproof}\end{addmargin}\qed}
\newenvironment{theorem}[2][Theorem]{\begin{trivlist}
\item[\hskip \labelsep {\bfseries #1} \hskip \labelsep {\bfseries #2.}]}{\end{trivlist}}
\newenvironment{example}[2][Example]{\begin{trivlist}
\item[\hskip \labelsep {\bfseries #1} \hskip \labelsep {\bfseries #2.}]}{\end{trivlist}}
\newenvironment{lemma}[2][Lemma]{\begin{trivlist}
\item[\hskip \labelsep {\bfseries #1} \hskip \labelsep {\bfseries #2.}]}{\end{trivlist}}
\newenvironment{exercise}[2][Exercise]{\begin{trivlist}
\item[\hskip \labelsep {\bfseries #1} \hskip \labelsep {\bfseries #2.}]}{\end{trivlist}}
\newenvironment{problem}[2][Problem]{\begin{trivlist}
\item[\hskip \labelsep {\bfseries #1} \hskip \labelsep {\bfseries #2.}]}{\end{trivlist}}
\newenvironment{corollary}[2][Corollary]{\begin{trivlist}
\item[\hskip \labelsep {\bfseries #1} \hskip \labelsep {\bfseries #2.}]}{\end{trivlist}}
\usepackage{fancyhdr,enumitem,changepage,url}
\pagestyle{fancy}
\author{Warren Atkison}
\date{\today}
\setlength{\headheight}{15pt}
\begin{document}
\fancyhf{}
\fancyhead[L]{Warren Atkison}
\fancyhead[C]{Special Assignment 4}
\fancyhead[R]{\today}
\fancyfoot[R]{\thepage}

\begin{problem}{1}
	This problem refers to Example 4 in Section 4.2. Explain why
	\[
		\int_{\Gamma} \bar{z}^2dz = \int_{\Gamma}(z^2 - 4xyi)dz = -4i\int_{\Gamma}xydz
	\]
	and evaluate the last integral using the parametrization given by the author.
\end{problem}
Let $z = x + iy$
\begin{align*}
	\int_{\Gamma} \bar{z}^2dz &= \int_{\Gamma} (x - iy)^2dz \\
				  &= \int_{\Gamma} (x^2 - y^2 - 2xyi)dz \\
				  &= \int_{\Gamma} [(x + iy)^2 - 4xyi]dz \\
				  &= \int_{\Gamma} (z^2 - 4xyi)dz \\
				  &= \int_{\Gamma} z^2dz -4i\int_{\Gamma} xydz
\end{align*}
Since $z^2$ is continous on $\mathbb{C}$, has an antiderivative throughout $\mathbb{C}$, and $\Gamma$ is a closed loop, by corollary 2 of Theorem 6 we know the our first integral is 0, leaving us with the desired result.
\[
	= -4i\int_{\Gamma} xydz
\]
The given parametrization for the 3 line segments of $\Gamma$ are
\begin{align*}
	\gamma_1: \quad z_1(t) &= x_1(t) + iy_1(t) = t & &(0 \le t \le 2), \\
	\gamma_2: \quad z_2(t) &= x_2(t) + iy_2(t) = 2 + ti & &(0 \le t \le 2), \\
	\gamma_3: \quad z_3(t) &= x_3(t) + iy_3(t) = -t(1 + i) & &(-2 \le t \le 0),
\end{align*}
so we have
\begin{align*}
	-4i\int_{\Gamma}xydz &= -4i\left(\int_{\gamma_1} xydz + \int_{\gamma_2} xydz + \int_{\gamma_3} xydz\right) \\
			     &= -4i\left(\int_0^2 x_1(t)y_1(t)z_1'(t)dt + \int_0^2 x_2(t)y_2(t)z_2'(t)dt + \int_{-2}^0 x_3(t)y_3(t)z_3'(t)dt\right) \\
			     &= -4i\left(0 + \int_0^2 2tidt + \int_{-2}^0 (-t)^2(-1 - i)dt\right) \\
			     &= -4i\left(2i\int_0^2 tdt - (1 + i)\int_{-2}^0 t^2dt\right) \\
			     &= -4i\left(2i\left[\frac{t^2}{2}\right]_0^2 - (1 + i)\left[\frac{t^3}{3}\right]_{-2}^0\right) \\
			     &= -4i\left(4i - (1 + i)\cdot\frac{8}{3}\right) \\
			     &= 16 + \frac{32i}{3} - \frac{32}{3} \\
			     &= \frac{16}{3} + \frac{32i}{3}
\end{align*}
\begin{problem}{2}
	Using the result from Exercise 6 in Section 4.3, we know that $\int_{C} \dfrac{1}{z - 1}dz = 2\pi i$, where $C$ is the circle $|z| = 2$ traversed once in the positive direction. By considering real and imaginary parts, use this result to evaluate
	\[
		\int_0^{2\pi} \frac{2 - \cos t}{5 - 4\cos t}dt
	\]
\end{problem}
Let $z = 2e^{it}$ for $0 \le t \le 2\pi$, then $dz = 2ie^{it}dt$ and
\begin{align*}
	\int_{C} \frac{1}{z - 1}dz &= \int_{0}^{2\pi} \frac{2ie^{it}}{2e^{it} - 1}dt \\
				   &= \int_0^{2\pi} \frac{2ie^{it}}{2e^{it} - 1} \cdot \frac{2e^{-it} - 1}{2e^{-it} - 1}dt \\
				   &= \int_0^{2\pi} \frac{4i - 2ie^{it}}{5 - 2e^{it} - 2e^{-it}}dt \\
				   &= \int_0^{2\pi} \frac{4i - 2i(\cos(t) + i\sin(t))}{5 - 4\cos(t)} \\
				   &= \int_0^{2\pi} \frac{2\sin(t)}{5 - 4\cos t}dt + 2i\int_{0}^{2\pi} \frac{2 - \cos t}{5 - 4\cos t}dt = 2\pi i \\
	\implies \int_0^{2\pi} \frac{2 - \cos t}{5 - 4\cos t}dt &= \pi
\end{align*}

\begin{problem}{3}
	Use partial fractions and the result of Exercise 4.3.6 to evaluate
	\[
		\int_{C} \frac{3z + 1}{(z - 1)(z^2 + 1)}dz
	\]
	where $C$ is the circle $|z-i| = \sqrt{3}$ traversed once in the positive direction.
\end{problem}
First we find the partial fractions of our function.
\begin{align*}
	\frac{3z + 1}{(z-1)(z+i)(z-i)} = \frac{A}{z-1} + \frac{B}{z+i} + \frac{C}{z-i}
\end{align*}
\begin{align*}
	A &= \frac{3(1) + 1}{1^2 + 1} = \frac{4}{2} = 2 \\
	B &= \frac{3(-i) + 1}{(-i-1)(-i-i)} = \frac{1 - 3i}{-2 + 2i} \cdot \frac{-2 - 2i}{-2 - 2i} = \frac{-8 + 4i}{8} = \frac{-2 + i}{2} \\
	C &= \frac{3(i) + 1}{(i-1)(i+i)} = \frac{1 + 3i}{-2 - 2i} \cdot \frac{-2 + 2i}{-2 + 2i} = \frac{-8 - 4i}{8} = \frac{-2 -i}{2}
\end{align*}
Since $|1 - i| = \sqrt{2} < \sqrt{3}$ and $|i - i| = 0 < \sqrt{3}$, both $z = 1$ and $z = i$ are in $C$, however $|-i - i| = 2 > \sqrt{3}$, so $z = -i$ is not in $C$. Therefore we only integrate around the points $z = 1$ and $z = i$. Let $C_0$ be a small circle around $z = 1$ and $C_1$ be the circle around $z = i$. Now we can evaluate our integral using our partial fraction decomposition and integrating around our small circles in the positive direction (which Theorem 13 allows us to do). 
\begin{align*}
	\int_{C} \frac{3z + 1}{(z - 1)(z^2 + 1)}dz &= \int_{C} \frac{3z + 1}{(z - 1)(z + i)(z - i)}dz \\
						   &= \int_{C_0} \frac{2}{z - 1}dz + \int_{C} \frac{-2 + i}{2(z + i)}dz + \int_{C_1} \frac{-2 -i}{2(z-i)}dz \\
						   &= 4\pi i + 0 + \pi i(-2 - i) \\
						   &= \pi + 2\pi i \\ 
						   &= \pi(1 + 2i)
\end{align*}
\end{document}
