\documentclass[12pt]{article}
\linespread{1.2}
\usepackage[margin=2cm]{geometry}
\usepackage[utf8]{inputenc}
\usepackage{amsfonts}
\usepackage{amsmath}
\usepackage{multicol}
\usepackage{amsthm}
\usepackage{amssymb,scrextend}
\usepackage{graphicx,tikz}
\newtheorem{dfn}{Definition}
\renewcommand{\qed}{\hfill$\blacksquare$}
\let\newproof\proof
\renewenvironment{proof}{\vspace{1em}\begin{addmargin}[2em]{0em}\begin{newproof}}{\end{newproof}\end{addmargin}\qed}
\newenvironment{theorem}[2][Theorem]{\begin{trivlist}
\item[\hskip \labelsep {\bfseries #1} \hskip \labelsep {\bfseries #2.}]}{\end{trivlist}}
\newenvironment{example}[2][Example]{\begin{trivlist}
\item[\hskip \labelsep {\bfseries #1} \hskip \labelsep {\bfseries #2.}]}{\end{trivlist}}
\newenvironment{lemma}[2][Lemma]{\begin{trivlist}
\item[\hskip \labelsep {\bfseries #1} \hskip \labelsep {\bfseries #2.}]}{\end{trivlist}}
\newenvironment{exercise}[2][Exercise]{\begin{trivlist}
\item[\hskip \labelsep {\bfseries #1} \hskip \labelsep {\bfseries #2.}]}{\end{trivlist}}
\newenvironment{problem}[2][Problem]{\begin{trivlist}
\item[\hskip \labelsep {\bfseries #1} \hskip \labelsep {\bfseries #2.}]}{\end{trivlist}}
\newenvironment{corollary}[2][Corollary]{\begin{trivlist}
\item[\hskip \labelsep {\bfseries #1} \hskip \labelsep {\bfseries #2.}]}{\end{trivlist}}
\usepackage{fancyhdr,enumitem,changepage,url}
\pagestyle{fancy}
\author{Warren Atkison}
\date{\today}
\setlength{\headheight}{15pt}
\begin{document}
\fancyhf{}
\fancyhead[L]{Warren Atkison}
\fancyhead[C]{Special Assignment 6}
\fancyhead[R]{\today}
\fancyfoot[R]{\thepage}

\begin{exercise}{5.4.3c}
	Find the radius of convergence of the following power series.
	\[
		\sum_{k=0}^{\infty} \left(2 + (-1)^k\right)^kz^k
	\]
\end{exercise}	
First we can find the sum of the series.
\begin{align*}
	\sum_{k=0}^{\infty} \left(2 + (-1)^k\right)^kz^k &= 1 + z + (3z)^2 + z^3 + (3z)^4 + \ldots \\
							 &= \sum_{k=0}^{\infty} (3z)^{2k} + \sum_{k=0}^{\infty} z^{2k+1} \\
							 &= \sum_{k=0}^{\infty} (9z^2)^k + z\sum_{k=0}^{\infty} (z^2)^k \\
							 &= \frac{1}{1 - 9z^2} + \frac{z}{1 - z^2}
\end{align*}
for $|9z^2| < 1$ and $|z^2| < 1$. We only care about the one which is more restrictive, so we have
\begin{align*}
	9|z|^2 &< 1 \implies |z| < \frac{1}{3} & |z|^2 < 1 \implies |z| < 1
\end{align*}
which gives us a radius of convergence of $1/3$.
\begin{exercise}{5.1.21}
	Let $0 < c < 1$. An increasingly lazy and asymmetric frog leaps one meter (from $z = 0$ to $z = 1$) on his first jump, $c$ meter on his second jump, $c^2$ meters on his third jump, and so on, each time turning exactly an angle $0 < \alpha < \pi/2$ to the left of his preceding flight path. Show the that frog eventually ends up on a circle that depends on $c$, but not $\alpha$.
\end{exercise}
\begin{proof}
	Let $S$ be the sum of the jumps of the frog and $z = e^{i\alpha}$. Since $|cz| = |c| < 1$, we have
	\begin{align*}
		S = 1 + cz + (cz)^2 + \ldots = \sum_{k=0}^{\infty} (cz)^{k} = \frac{1}{1 - cz}
	\end{align*}
	Consider the following quantity.
	\begin{align*}
		|(1 - c^2)S - 1|^2 &= \left(\frac{1 - c^2}{1 - cz} - 1\right)\left(\frac{1 - c^2}{1 - c/z} - 1\right) \\
				   &= \left(\frac{1 - c^2}{1 - cz} - 1\right)\left(\frac{z - c^2z}{z - c} - 1\right) \\
				   &= \frac{z(1 - c^2)(1 - c^2)}{(1 - cz)(z - c)} - \frac{1 - c^2}{1 - cz} - \frac{z - c^2z}{z - c} + 1 \\
				   &= \frac{z(1 - c^2)(1 - c^2)}{(1 - cz)(z - c)} - \frac{(1 - c^2)(z - c)}{(1 - cz)(z - c)} - \frac{(z - c^2z)(1 - cz)}{(z - c)(1 - cz)} + 1 \\
				   &= \frac{z - 2c^2z + zc^4 - z + c + c^2z - c^3 - z + cz^2 +c^2z - c^3z^2 + z - cz^2 - c + c^2z}{(z - c)(1 - cz)} \\
				   &= \frac{c^2z + zc^4 - c^3 - c^3z^2}{(z - c)(1 - cz)} \\
				   &= \frac{c^2(z + zc^2 - c - cz^2)}{(z - c)(1 - cz)} \\
				   &= \frac{c^2(z(1 - cz) - c(1 - cz))}{(z - c)(1 - cz)} \\
				   &= c^2 \\
		\implies |(1 - c^2)S - 1| &= c
	\end{align*}
	Then we have
	\[
		\left|S - \frac{1}{1 - c^2}\right| = \frac{c}{1 - c^2}
	\]
	which gives us a center at $\dfrac{1}{1 - c^2}$ and a radius of $\dfrac{c}{1 - c^2}$
\end{proof}
\begin{problem}{3}
	Show that the function $f$ defined by the power series $f(z) = \sum\limits_{k=0}^{\infty}\frac{(-1)^k}{4^k(k!)^2}z^{2k}$ satisfies the differential equation $zf''(z) + f'(z) + zf(z) = 0$.
\end{problem}
\begin{proof}
	Fist consider
	\begin{align*}
		f'(z) &= \sum_{k=0}^{\infty} \frac{2k(-1)^k}{4^k(k!)^2}z^{2k-1} \\
		f''(z) &= \sum_{k=0}^{\infty} \frac{2k(2k - 1)(-1)^k}{4^k(k!)^2}z^{2k - 2}.
	\end{align*}
	so
	\begin{align*}
		zf''(z) + f'(z) + zf(z) &= z\sum_{k=0}^{\infty} \frac{2k(2k - 1)(-1)^k}{4^k(k!)^2}z^{2k - 2} + \sum_{k=0}^{\infty} \frac{2k(-1)^k}{4^k(k!)^2}z^{2k-1} + z\sum_{k=0}^{\infty}\frac{(-1)^k}{4^k(k!)^2}z^{2k} \\
		&= \sum_{k=0}^{\infty} \left(\frac{2k(2k - 1)(-1)^k}{4^k(k!)^2} + \frac{2k(-1)^k}{4^k(k!)^2}\right)z^{2k - 1} + \sum_{k=0}^{\infty}\frac{(-1)^{k}}{4^k(k!)^2}z^{2k + 1} \\
		&= \sum_{k=1}^{\infty} \left(\frac{2k(2k - 1)(-1)^k}{4^k(k!)^2} + \frac{2k(-1)^k}{4^k(k!)^2}\right)z^{2k - 1} + \sum_{k=1}^{\infty}\frac{(-1)^{k-1}}{4^{k-1}((k-1)!)^2}z^{2k - 1} \\
		&= \sum_{k=1}^{\infty} \left(\frac{2k(2k - 1)(-1)^k}{4^k(k!)^2} + \frac{2k(-1)^k}{4^k(k!)^2} + \frac{(-1)^{k-1}}{4^{k-1}((k-1)!)^2}\right)z^{2k - 1} \\
		&= \sum_{k=1}^{\infty} \left(\frac{2k(2k - 1)(-1)^k}{4^k(k!)^2} + \frac{2k(-1)^k}{4^k(k!)^2} - \frac{4k^2(-1)^{k}}{4^{k}(k!)^2}\right)z^{2k - 1} \\
		&= \sum_{k=1}^{\infty} \frac{(-1)^k(4k^2 - 2k + 2k - 4k^2)}{4^k(k!)^2}z^{2k-1} \\
		&= 0
	\end{align*}
\end{proof}
\begin{problem}{4}
	Consider the function $g(z) = \dfrac{1}{(z+2)(z-3)}$. Find the Laurent series for the function $g$ in each of the following domains:
	\begin{itemize}
		\item[(a)] $0 < |z| < 2$ \\
			First note:
			\[
				\frac{1}{(z + 2)(z - 3)} = \frac{1}{5(z - 3)}-\frac{1}{5(z + 2)} 
			\]
			Then for $|z| < 2$ we have
			\begin{align*}
				\frac{1}{5(z - 3)} &= -\frac{1}{15}\cdot\frac{1}{1 - z/3} = -\frac{1}{15}\sum_{k=0}^{\infty} \left(\frac{z}{3}\right)^k = -\sum_{k=0}^{\infty} \frac{z^k}{5\cdot 3^{k+1}}
			\end{align*}
			and
			\begin{align*}
				\frac{1}{5(z + 2)} &= \frac{1}{10}\cdot\frac{1}{1 - (-z)/2} = \frac{1}{10}\sum_{k=0}^{\infty} (-1)^k\left(\frac{z}{2}\right)^k = \sum_{k=0}^{\infty} \frac{(-1)^kz^k}{5\cdot2^{k+1}}
			\end{align*}
			so
			\begin{align*}
				\frac{1}{(z+2)(z-3)} = \sum_{k=0}^{\infty} \left(-\frac{1}{5\cdot3^{k+1}} - \frac{(-1)^k}{5\cdot2^{k+1}}\right)z^k.
			\end{align*}
		\item[(b)] $2 < |z| < 3$ \\
			For $\dfrac{1}{5(z - 3)}$ our equation is still valid, but we have
			\begin{align*}
				\frac{1}{5(z+2)} = \frac{1}{5z}\cdot\frac{1}{1 - (-2)/z} = \frac{1}{5z}\sum_{k=0}^{\infty} (-1)^k\left(\frac{2}{z}\right)^k = \sum_{k=0}^{\infty} \frac{(-1)^k2^k}{5z^{k+1}} 
			\end{align*}
			so
			\begin{align*}
				\frac{1}{(z+2)(z-3)} = -\sum_{k=0}^{\infty} \frac{z^k}{5\cdot3^{k+1}} - \sum_{k=0}^{\infty} \frac{(-1)^k2^k}{5z^{k+1}}.
			\end{align*}
		\item[(c)] $|z - 3| > 5$ \\
			Since we are centering our series at $z = 3$ \ldots
			\begin{align*}
				\frac{1}{5(z+2)} &= \frac{1}{5}\cdot\frac{1}{(z - 3) + 5} = \frac{1}{5(z - 3)} \cdot \frac{1}{1 - (-5)/(z - 3)} = \frac{1}{5(z - 3)}\sum_{k=0}^{\infty} (-1)\left(\frac{5}{(z - 3)}\right)^k \\
						 &= \sum_{k=0}^{\infty} \frac{(-1)^k5^{k-1}}{(z - 3)^{k + 1}}
			\end{align*}
			so
	\[
		\frac{1}{(z +2)(z-3)} = \frac{1}{5(z - 3)} - \sum_{k=0}^{\infty} \frac{(-1)^k5^{k-1}}{(z - 3)^{k+1}}
	\]
		\item[(d)]
			$|z| > 3$
			\begin{align*}
				\frac{1}{5(z-3)} &= \frac{1}{5z} \cdot \frac{1}{1 - 3/z} = \frac{1}{5z}\sum_{k=0}^{\infty} \left(\frac{3}{z}\right)^k = \sum_{k=0}^{\infty} \frac{3^k}{5z^{k+1}}
			\end{align*}
	\end{itemize}

\end{problem}
\end{document}

